.

counter_machine/counter_machine.thy
@@ -10,7 +10,6 @@ type_synonym INPUT_A = bool
 type_synonym INPUT_B = bool
 type_synonym OUT = "nat option"
 type_synonym COUNT = nat
-
 type_synonym STATE= State
 
 definition INIT_NODE:: "STATE" where
@@ -30,10 +29,82 @@ fun t:: "(INPUT_A \<times> INPUT_B \<times> STATE \<times> COUNT) \<Rightarrow> 
 "t(False, True, S, C) = ((Some C), S, 0::nat)"|
 "t(False,False, S, C) = (None, S, C)"
 
-definition paths:: "(nat \<Rightarrow> STEP) set" where
-"paths \<equiv> {p::(nat\<Rightarrow>STEP). STATE(p 0) = INIT_NODE \<and> (\<forall>n. t(I_A(p(n)), I_B (p(n)), STATE(p(n)), COUNT(p(n))) = (OUT(p(n)), STATE(p(Suc n)), COUNT(p(Suc n))))}"
+type_synonym path = "nat \<Rightarrow> STEP"
+
+definition paths:: "path set" where
+"paths \<equiv> {p::path. STATE(p 0) = INIT_NODE \<and> (\<forall>n. t(I_A(p(n)), I_B (p(n)), STATE(p(n)), COUNT(p(n))) = (OUT(p(n)), STATE(p(Suc n)), COUNT(p(Suc n))))}"
 
 
+definition simple_path:: "path" where
+"simple_path n = \<lparr>I_A=True,I_B=True, OUT= Some(1), STATE=INIT_NODE, COUNT= 0\<rparr>"
+
+
+(*prove that paths is not empty*)
+
+lemma "paths \<noteq> {}"
+proof
+  assume init_assm: "paths = {}"
+  show "False"
+  proof-
+    fix n
+    have 1: "simple_path n = \<lparr>I_A=True,I_B=True, OUT= Some(1), STATE=INIT_NODE, COUNT= 0\<rparr>" using simple_path_def by simp
+    (*show that the simple path has props of a path*)
+    then have s_p_0: "simple_path 0 =  \<lparr>I_A=True,I_B=True, OUT= Some(1), STATE=INIT_NODE, COUNT= 0\<rparr>" using simple_path_def by blast
+    then have cond1: "STATE(simple_path 0) = INIT_NODE" using s_p_0 by simp
+    have RHS: "(OUT(simple_path n), STATE(simple_path (Suc n)), COUNT(simple_path(Suc n))) = (Some(1),INIT_NODE, 0)" using simple_path_def by simp
+    hence cond2: "\<forall>n. t(I_A(simple_path (n)), I_B (simple_path (n)), STATE(simple_path (n)), COUNT(simple_path (n))) = (OUT(simple_path n), STATE(simple_path (Suc n)), COUNT(simple_path(Suc n)))"
+    by (simp add: simple_path_def)
+    hence cond1_cond2: "STATE(simple_path 0) = INIT_NODE \<and> (\<forall>n. t(I_A(simple_path (n)), I_B (simple_path (n)), STATE(simple_path (n)), COUNT(simple_path (n))) = (OUT(simple_path n), STATE(simple_path (Suc n)), COUNT(simple_path(Suc n))))"
+      using cond1 cond2 by blast
+    thus "False" using init_assm paths_def by fastforce
+  qed
+qed
+
+
+fun count:: "path \<Rightarrow> nat \<Rightarrow> nat \<Rightarrow> nat" where
+"count p n 0 = 0"|
+"count p n (Suc n') = (count p n n') + (if(I_A(p (Suc (n' + n))) = True) then 1 else 0 )"
+
+value "count simple_path 0 "
+
+lemma "count simple_path 0 n = n"
+proof(induction n)
+  case 0
+  then show ?case
+    by auto
+next
+  case (Suc n)
+  have init: "count simple_path 0 (Suc n) = count simple_path 0 n + (if(I_A(simple_path(Suc n)) = True) then 1 else 0 )" by auto
+  moreover have "... = n + (if(I_A(simple_path(Suc n)) = True) then 1 else 0 )" using Suc by simp
+  moreover have "... = n + (if(True) then 1 else 0)" using simple_path_def by simp
+  moreover have "... = n + 1" by auto
+  moreover have "... = Suc n" by auto
+  ultimately show ?case by auto
+qed
+
+
+(*"paths \<equiv> {p::path. STATE(p 0) = INIT_NODE \<and> (\<forall>n. t(I_A(p(n)), I_B (p(n)), STATE(p(n)), COUNT(p(n))) = (OUT(p(n)), STATE(p(Suc n)), COUNT(p(Suc n))))}"*)
+lemma "\<forall>p \<in> paths. \<forall>n<n'. I_A(p n) = True \<and> I_B(p n') = True \<and> (\<forall>m. m \<in> {n<..<n'} \<longrightarrow> OUT(p m) = None) \<longrightarrow> OUT(p n') = Some(count p n (n'- n))"
+proof
+  fix p
+  assume base: "p \<in> paths"
+  show "\<forall>n<n'. I_A (p n) = True \<and> I_B (p n') = True \<and> (\<forall>m. m \<in> {n<..<n'} \<longrightarrow> OUT (p m) = None) \<longrightarrow> OUT (p n') = Some (count p n (n' - n))"
+  proof(induction n')
+    case 0
+    then show ?case by auto
+  next
+    case (Suc n')
+    (**)
+    show ?case
+    proof
+      assume LHS: "\<forall>n<Suc n'. I_A (p n) = True \<and> I_B (p (Suc n')) = True \<and> (\<forall>m. m \<in> {n<..<Suc n'} \<longrightarrow> OUT (p m) = None)"
+      then consider "Suc n = Suc n'"| "Suc n \<noteq> Suc n'" by auto
+      then show "OUT (p (Suc n')) = Some(count p n (Suc n'- n))"
+    qed
+  qed
+  
+  qed
+qed
 
 
 end
